examples/unit-tests/insertionsort.fst
@@ -1,5 +1,5 @@
 (*
-   Copyright 2008-2014 Nikhil Swamy and Microsoft Research
+   Copyright 2008-2014 Nikhil Swamy, Chantal Keller and Microsoft Research
 
    Licensed under the Apache License, Version 2.0 (the "License");
    you may not use this file except in compliance with the License.
@@ -18,17 +18,18 @@
 module InsertionSort
 open Prims.PURE
 
-
-(* An effect abbreviation for a lemma *)
-(*ghost*) effect Fact ('res:Type) ('p:Type) = Pure 'res True (fun r => 'p)
-
-
 (* Check that a list is sorted *)
 val sorted: list int -> Tot bool
 let rec sorted l = match l with
     | [] -> true
     | [x] -> true
-    | x::y::xs -> (x < y) && (sorted (y::xs))
+    | x::y::xs -> x <= y && sorted (y::xs)
+
+val test_sorted: x:int -> l:list int -> Fact unit ((sorted (x::l) /\ is_Cons l) ==> x <= Cons.hd l)
+let test_sorted x l = ()
+
+val test_sorted2: unit -> Tot (m:list int{sorted m})
+let test_sorted2 () = Nil
 
 (* Fact about sorted *)
 val mem: 'a -> list 'a -> Tot bool
@@ -37,19 +38,24 @@ let rec mem a l = match l with
   | hd::tl -> hd=a || mem a tl
 
 val sorted_smaller: x:int -> y:int -> l:list int ->
-                    Fact unit (sorted (x::l) ==> mem y l ==> x < y)
+                    Fact unit (sorted (x::l) /\ mem y l ==> x <= y)
 let rec sorted_smaller x y l = match l with
     | [] -> ()
     | z::zs -> if z=y then () else sorted_smaller x y zs
 
-(* Insertion in a sorted list: does not work at such for now *)
-val insert : int -> l:list int{sorted l == true} -> Tot (l':list int{sorted l' == true})
-let rec insert y l = match l with
-    | [] -> [y]
-    | x::xs -> if y < x then y::l else x::(insert y xs)
+val insert : i:int -> l:list int{sorted l} -> Tot (m:list int{sorted m /\ (forall x. mem x m <==> x==i \/ mem x l)})
+let rec insert i l = match l with
+  | [] -> [i]
+  | hd::tl ->
+     if i <= hd
+     then i::l
+     else let i_tl = insert i tl in 
+          let (z::_) = i_tl in
+          sorted_smaller hd z tl; (* need to call the lemma explicitly, currently *)
+          hd::i_tl
 
 (* Insertion sort *)
-val sort : list int -> Tot (l:list int{sorted l == true})
+val sort : l:list int -> Tot (m:list int{sorted m /\ (forall x. mem x l == mem x m)})
 let rec sort l = match l with
     | [] -> []
     | x::xs -> insert x (sort xs)
